add tests in setbit/verif.v

examples/setbit/verif.v
@@ -5,14 +5,46 @@ Import ListNotations.
 Require Import p4ast.
 
 Require Import Petr4.Semantics.
+Require Import Petr4.Trans.
+
+Definition prog2 := ltac:(let x := eval compute in (transform_prog NoInfo prog) in exact x).
 
 Opaque IdentMap.empty IdentMap.set PathMap.empty PathMap.set.
 
-Definition ge := ltac:(let x := eval compute in (load_prog prog) in exact x).
+Definition ge := ltac:(let x := eval compute in (load_prog prog2) in exact x).
 
-Definition init_mem := ltac:(let x := eval compute in (instantiate_prog prog) in exact x).
+Definition init_mem := ltac:(let x := eval compute in (instantiate_prog prog2) in exact x).
 
 Transparent IdentMap.empty IdentMap.set PathMap.empty PathMap.set.
+
+Definition standard_init_mem :=
+  PathMap.set [{| P4String.tags := NoInfo; str := "main" |}; {| P4String.tags := NoInfo; str := "dep" |}]
+    (MClass {| P4String.tags := NoInfo; str := "MyDeparser" |})
+    (PathMap.set
+       [{| P4String.tags := NoInfo; str := "main" |}; {| P4String.tags := NoInfo; str := "ck" |}]
+       (MClass {| P4String.tags := NoInfo; str := "MyComputeChecksum" |})
+       (PathMap.set
+          [{| P4String.tags := NoInfo; str := "main" |}; {| P4String.tags := NoInfo; str := "eg" |}]
+          (MClass {| P4String.tags := NoInfo; str := "MyEgress" |})
+          (PathMap.set
+             [{| P4String.tags := NoInfo; str := "main" |}; {| P4String.tags := NoInfo; str := "ig" |}]
+             (MClass {| P4String.tags := NoInfo; str := "MyIngress" |})
+             (PathMap.set
+                [{| P4String.tags := NoInfo; str := "main" |}; {| P4String.tags := NoInfo; str := "ig" |};
+                {| P4String.tags := NoInfo; str := "incr" |}]
+                (MClass {| P4String.tags := NoInfo; str := "Increment" |})
+                (PathMap.set
+                   [{| P4String.tags := NoInfo; str := "main" |};
+                   {| P4String.tags := NoInfo; str := "vr" |}]
+                   (MClass {| P4String.tags := NoInfo; str := "MyVerifyChecksum" |})
+                   (PathMap.set
+                      [{| P4String.tags := NoInfo; str := "main" |};
+                      {| P4String.tags := NoInfo; str := "p" |}]
+                      (MClass {| P4String.tags := NoInfo; str := "MyParser" |}) PathMap.empty)))))).
+
+Goal init_mem = standard_init_mem.
+reflexivity.
+Qed.
 
 Definition myStatement := MkStatement NoInfo
               (StatAssignment
@@ -40,11 +72,11 @@ Definition myStatement := MkStatement NoInfo
 
 Definition _var := {| stags := NoInfo; str := "var" |}.
 
-Definition myEnv := IdentMap.set IdentMap.empty _var (Instance (BareName _var)).
+Definition myEnv := IdentMap.set _var (Instance [_var]) IdentMap.empty.
 
-Instance external : External := Build_External unit.
+Instance external : @External Info. Admitted. (*  := Build_External unit. *)
 
 Lemma property1: forall ge this decls m m' exts,
-    exec_stmt ge this decls myEnv (m, exts) myStatement (m', exts) Out_normal ->
-    PathMap.get m (name_cons this _var) = Some (MVal (VInt 2)) ->
-    PathMap.get m' (name_cons this _var) = Some (MVal (VInt 3)).
+    exec_stmt ge this decls myEnv init_mem (m, exts) myStatement (m', exts) Out_normal ->
+    PathMap.get (name_cons this _var) m = Some (ValBaseInteger 2) ->
+    PathMap.get (name_cons this _var) m' = Some (ValBaseInteger 3).
